Name: Bryant Har

NetID: bjh254

Derivation for state update: 

$x_t$ derivation:

$$
\begin{align*}
&\int_{x_{t-1}}^{x_t} dx =\int_{t}^{t+ \Delta t} v \cos \theta dt  \\
&x_{t}-x_{t-1}=\int_{\theta_{t-1}}^{\theta_t} \frac{L}{\tan \alpha} \cos \theta d\theta\\
&x_{t}-x_{t-1}=\frac{L}{\tan \alpha} (\sin \theta_{t}-\sin \theta_{t-1})\\
&x_{t}=x_{t-1}+\frac{L}{\tan \alpha} (\sin (\theta_{t-1}+\frac{v}{L} \tan \alpha \Delta t)-\sin \theta_{t-1})
\end{align*}
$$
u-sub for theta in line 2.
Use line 3 or line 4 as solution if dt is/is not kept. Line 4 was used for my code.
$y_t$ derivation:

$$
\begin{align*}
&\int_{y_{t-1}}^{y_t} dx =\int_{t}^{t+ \Delta t} v \sin \theta dt  \\
&y_{t}-y_{t-1}=\int_{\theta_{t-1}}^{\theta_t} \frac{L}{\tan \alpha} \sin \theta d\theta\\
&y_{t}-y_{t-1}=\frac{L}{\tan \alpha} (\cos \theta_{t-1}-\cos \theta_{t})\\
&y_{t}=y_{t-1}+\frac{L}{\tan \alpha} (\cos \theta_{t-1}-\cos (\theta_{t-1}+\frac{v}{L} \tan \alpha \Delta t))
\end{align*}
$$
u-sub for theta in line 2.
Use line 3 or line 4 as solution if dt is/is not kept. Line 4 was used for my code.
